Edit some comments.

automatic.v
@@ -6,27 +6,6 @@ From larith Require Import tactics notations utilities vector.
 From larith Require Import formulae automata regular.
 Import Nat ListNotations.
 
-(* Finite-length vectors form a finite alphabet. *)
-Section Finite_vector_alphabet.
-
-Fixpoint enumerate_vectors n : list (vec n) :=
-  match n with
-  | 0 => [⟨⟩]
-  | S m =>
-    let vs := enumerate_vectors m in
-    map (Vector.cons _ false m) vs ++
-    map (Vector.cons _ true m) vs
-  end.
-
-Theorem enumerate_vectors_spec n (v : vec n) :
-  In v (enumerate_vectors n).
-Proof.
-induction v; simpl. now left.
-apply in_app_iff; destruct h; [right|left]; apply in_map, IHv.
-Qed.
-
-End Finite_vector_alphabet.
-
 (* Algorithm for deciding first-order realizability using finite automata. *)
 Section Decide_wff_using_automata.
 
